update FlatImp semantics, now MMIO compiles up to where it might be interesting

bedrock2/src/Semantics.v
@@ -2,33 +2,9 @@ Require Import coqutil.sanity coqutil.Macros.subst coqutil.Macros.unique.
 Require Import coqutil.Datatypes.PrimitivePair coqutil.Datatypes.HList.
 Require Import bedrock2.Notations bedrock2.Syntax coqutil.Map.Interface.
 Require Import BinIntDef coqutil.Word.Interface coqutil.Word.LittleEndian.
+Require Export bedrock2.Memory.
 
 Require Coq.Lists.List.
-
-(* TODO: moveme *)
-Module List.
-  Section WithA.
-    Context {A : Type}.
-    Fixpoint option_all (xs : list (option A)) {struct xs} : option (list A) :=
-      match xs with
-      | nil => Some nil
-      | cons ox xs =>
-        match ox, option_all xs with
-        | Some x, Some ys => Some (cons x ys)
-        | _ , _ => None
-        end
-      end.
-
-    Section WithStep.
-      Context (step : A -> A).
-      Fixpoint unfoldn (n : nat) (start : A) :=
-        match n with
-        | 0%nat => nil
-        | S n => cons start (unfoldn n (step start))
-        end.
-    End WithStep.
-  End WithA.
-End List.
 
 Class parameters := {
   syntax :> Syntax.parameters;
@@ -60,26 +36,6 @@ Class parameters := {
 
 Section semantics.
   Context {pp : unique! parameters}.
-  Definition bytes_per sz :=
-    match sz with
-      | access_size.one => 1 | access_size.two => 2 | access_size.four => 4
-      | access_size.word => Z.to_nat (Z.div (Z.add width 7) 8)
-    end%nat.
-
-  Definition footprint(a: word)(sz: access_size) :=
-    List.unfoldn (fun w => word.add w (word.of_Z 1)) (bytes_per sz) a.
-  Definition load(sz: access_size)(m: mem)(a: word): option word :=
-    'Some bs <- List.option_all (List.map (map.get m) (footprint a sz)) | None ;
-    Some (word.of_Z (LittleEndian.combine _ (tuple.of_list bs))).
-  Definition unchecked_store(sz: access_size)(m: mem)(a: word)(v: word) : option mem :=
-    map.putmany_of_list
-      (footprint a sz)
-      (tuple.to_list (LittleEndian.split (bytes_per sz) (word.unsigned v)))
-      m.
-  Definition store(sz: access_size)(m: mem)(a: word)(v: word): option mem :=
-    'Some _ <- load sz m a | None;
-    unchecked_store sz m a v.
-
   Section WithMemAndLocals.
     Context (m : mem) (l : locals).
     Fixpoint eval_expr (e : expr) : option word :=
@@ -139,7 +95,7 @@ Module exec. Section WithEnv.
     (_ : eval_expr m l e = Some (word.of_Z 0))
     (_ : post t m l)
     : exec (cmd.while e c) t m l post
-  | while_true e c 
+  | while_true e c
       t m l post
       v (_ : eval_expr m l e  = Some v)
       (_ : v <> word.of_Z 0)
@@ -158,7 +114,7 @@ Module exec. Section WithEnv.
             map.putmany_of_list binds retvs l = Some l' /\
             post t' m' l')
     : exec (cmd.call binds fname arges) t m l post
-  | interact binds action arges 
+  | interact binds action arges
              t m l post
       args (_ : List.option_all (List.map (eval_expr m l) arges) = Some args)
       mid (_ : ext_spec t m action args mid)
