bedrock2/src/Memory.v
@@ -1,0 +1,55 @@
+Require Coq.Lists.List.
+Require Import coqutil.sanity.
+Require Import coqutil.Datatypes.PrimitivePair coqutil.Datatypes.HList.
+Require Import bedrock2.Notations bedrock2.Syntax coqutil.Map.Interface.
+Require Import BinIntDef coqutil.Word.Interface coqutil.Word.LittleEndian.
+
+(* TODO: moveme *)
+Module List.
+  Section WithA.
+    Context {A : Type}.
+    Fixpoint option_all (xs : list (option A)) {struct xs} : option (list A) :=
+      match xs with
+      | nil => Some nil
+      | cons ox xs =>
+        match ox, option_all xs with
+        | Some x, Some ys => Some (cons x ys)
+        | _ , _ => None
+        end
+      end.
+
+    Section WithStep.
+      Context (step : A -> A).
+      Fixpoint unfoldn (n : nat) (start : A) :=
+        match n with
+        | 0%nat => nil
+        | S n => cons start (unfoldn n (step start))
+        end.
+    End WithStep.
+  End WithA.
+End List.
+
+Section Memory.
+  Context {byte: word 8} {width: Z} {word: word width} {mem: map.map word byte}.
+
+  Definition bytes_per sz :=
+    match sz with
+      | access_size.one => 1 | access_size.two => 2 | access_size.four => 4
+      | access_size.word => Z.to_nat (Z.div (Z.add width 7) 8)
+    end%nat.
+
+  Definition footprint(a: word)(sz: access_size) :=
+    List.unfoldn (fun w => word.add w (word.of_Z 1)) (bytes_per sz) a.
+  Definition load(sz: access_size)(m: mem)(a: word): option word :=
+    'Some bs <- List.option_all (List.map (map.get m) (footprint a sz)) | None ;
+    Some (word.of_Z (LittleEndian.combine _ (tuple.of_list bs))).
+  Definition unchecked_store(sz: access_size)(m: mem)(a: word)(v: word) : option mem :=
+    map.putmany_of_list
+      (footprint a sz)
+      (tuple.to_list (LittleEndian.split (bytes_per sz) (word.unsigned v)))
+      m.
+  Definition store(sz: access_size)(m: mem)(a: word)(v: word): option mem :=
+    'Some _ <- load sz m a | None;
+    unchecked_store sz m a v.
+
+End Memory.
