compiler/src/containsProgram.v
@@ -8,7 +8,6 @@ Require Import riscv.Decode.
 Require Import riscv.Run.
 Require Import riscv.Memory.
 Require Import coqutil.Decidable.
-Require compiler.Memory.
 Require Import Coq.Program.Tactics.
 Require Import riscv.InstructionCoercions.
 Require Import riscv.AxiomaticRiscv.
