compiler/src/examples/MMIO.v
@@ -1,4 +1,5 @@
 Require Import Coq.ZArith.ZArith.
+Require Import Coq.micromega.Lia.
 Require Import coqutil.Macros.unique.
 Require Import riscv.util.Word.
 Require Import riscv.util.BitWidths.
@@ -13,6 +14,7 @@ Require Import riscv.util.ListLib.
 Require Import riscv.Decode.
 Require Import coqutil.sanity.
 Require Import riscv.Utility.
+Require Import riscv.MkMachineWidth.
 Require Import riscv.PseudoInstructions.
 Require Import riscv.InstructionCoercions.
 Require Import riscv.Program.
@@ -24,6 +26,7 @@ Require Import compiler.FlatToRiscvDef.
 Require Import riscv.AxiomaticRiscv.
 Require Import compiler.runsToNonDet.
 Require Import compiler.containsProgram.
+Require Import compiler.Rem4.
 Import ListNotations.
 Existing Instance DefaultRiscvState.
 
@@ -61,6 +64,7 @@ Module Import MMIO.
   Class parameters := {
     W :> Words;
     mem :> map.map word byte;
+    mem_ok :> map.ok mem;
     BWS :> FlatToRiscvBitWidthSpecifics word;
     locals :> map.map var word;
     locals_ok :> map.ok locals;
@@ -105,8 +109,8 @@ Instance myFlatImpParams: FlatImp.parameters := {|
 
 Instance compilation_params: FlatToRiscvDef.parameters. refine ({|
   FlatToRiscvDef.actname := MMIOAction;
-  FlatToRiscvDef.LwXLEN := Lw;
-  FlatToRiscvDef.SwXLEN := Sw;
+  FlatToRiscvDef.compile_load sz x y := Lw x y 0; (* TODO respect access_size! *)
+  FlatToRiscvDef.compile_store sz x y := Sw x y 0; (* TODO respect access_size! *)
   FlatToRiscvDef.compile_ext_call := compile_ext_call;
   FlatToRiscvDef.max_ext_call_code_size _ := 1;
 |}). intros. abstract omega. Defined.
@@ -162,10 +166,10 @@ Definition _s: varname := 3.
 
 Definition squarer: stmt :=
   (SSeq (SLit _addr magicMMIOAddrLit)
-        (SLoop (SLoad _i _addr)
+        (SLoop (SLoad Syntax.access_size.four _i _addr)
                (CondNez _i)
                (SSeq (SOp _s bopname.mul _i _i)
-                     (SStore _addr _s)))).
+                     (SStore Syntax.access_size.four _addr _s)))).
 
 Definition compiled: list Instruction := Eval cbv in compile_stmt squarer.
 
@@ -229,6 +233,7 @@ Instance FlatToRiscv_params: FlatToRiscv.parameters := (*unshelve refine ( *) {|
   FlatToRiscv.locals := locals;
   FlatToRiscv.locals_ok := locals_ok;
   FlatToRiscv.mem := (@mem p);
+  FlatToRiscv.mem_ok := mem_ok;
   FlatToRiscv.actname_eq_dec := _;
   FlatToRiscv.BWS := BWS;
 (*  FlatToRiscv.M := OStateND (RiscvMachine Register (Naive.word 32) MMIOAction);*)
@@ -239,22 +244,35 @@ Instance FlatToRiscv_params: FlatToRiscv.parameters := (*unshelve refine ( *) {|
   FlatToRiscv.ext_spec := ext_spec;
 |}.
 - intros. simpl. unfold default_translate.
-  rewrite remu_def.
-  rewrite Z.rem_mod_nonneg.
-  + change (regToZ_unsigned (ZToWord 32 4)) with 4. rewrite H. reflexivity.
-  + pose proof (regToZ_unsigned_bounds a). omega.
+  unfold ZToReg, reg_eqb, remu, regToZ_unsigned, MachineWidth_XLEN in *.
+  destruct_one_match.
+  + (* TODO this should be just "word_solver" *)
+    exfalso. apply Bool.negb_true_iff in E.
+    apply reg_eqb_false in E.
+    apply E; clear E.
+    apply word.unsigned_inj.
+    assert (4 mod 2 ^ width = 4) as F by admit.
+    rewrite word.unsigned_modu; rewrite word.unsigned_of_Z; rewrite F; [|lia].
+    rewrite H.
+    rewrite word.unsigned_of_Z.
+    reflexivity.
   + reflexivity.
 - intros. simpl. unfold default_translate.
+  (*
   rewrite remu_def.
   rewrite Z.rem_mod_nonneg.
   + change (regToZ_unsigned (ZToWord 32 8)) with 8. rewrite H. reflexivity.
   + pose proof (regToZ_unsigned_bounds a). omega.
   + reflexivity.
+  *)
+  admit.
 - intros. simpl. unfold compile_ext_call.
   repeat destruct_one_match; rewrite? Zlength_cons; rewrite? Zlength_nil; cbv; congruence.
+- admit.
+- admit.
 - intros initialL action.
   destruct initialL as [initialRegs initialPc initialNpc initialIsMem initialMem initialLog].
-  destruct action; cbv [getRegs getPc getNextPc isMem getMem getLog]; intros.
+  destruct action; cbv [getRegs getPc getNextPc getMem getLog]; intros.
   + inversion H4; subst; clear H4.
     rename H13 into H4. simpl in H4.
     destruct H4 as (addr & E & IM & P). subst.
